Superposition_Calculus/Abstract_Substitution/Variable_Substitution.thy
@@ -1,0 +1,54 @@
+theory Variable_Substitution
+  imports Abstract_Substitution
+begin
+
+(* TODO: Better name?: functional substitution *)
+locale variable_substitution = basic_substitution _ _ subst "\<lambda>a.  vars a = {}"
+  for subst :: "'value \<Rightarrow> ('x \<Rightarrow> 'subvalue) \<Rightarrow> 'value" (infixl "\<cdot>" 70) and
+    (* TODO: set \<rightarrow> fset *)
+      vars :: "'value \<Rightarrow> 'x set" +
+  assumes
+    subst_eq: "\<And>a \<sigma> \<tau>. (\<And>x. x \<in> vars a \<Longrightarrow> \<sigma> x = \<tau> x) \<Longrightarrow> a \<cdot> \<sigma> = a \<cdot> \<tau>" and
+    finite_vars [simp]: "\<And>a. finite (vars a)"
+begin
+
+abbreviation is_ground where "is_ground a \<equiv> vars a = {}"
+
+lemma subst_reduntant_upd [simp]:
+  assumes "var \<notin> vars a"
+  shows "a \<cdot> \<sigma>(var := update) = a \<cdot> \<sigma>"
+  using assms subst_eq by fastforce
+
+lemma subst_reduntant_if [simp]: 
+  assumes "vars a \<subseteq> vars'"
+  shows "a \<cdot> (\<lambda>var. if var \<in> vars' then \<sigma> var else \<sigma>' var) = a \<cdot> \<sigma>"
+  using assms
+  by (smt (verit, ccfv_SIG) subsetD subst_eq)
+
+lemma subst_reduntant_if' [simp]: 
+  assumes "vars a \<inter> vars' = {}"  
+  shows "a \<cdot> (\<lambda>var. if var \<in> vars' then \<sigma>' var else \<sigma> var) = a \<cdot> \<sigma>"
+  using assms
+  by (smt (verit, ccfv_SIG) disjoint_iff_not_equal subst_eq)
+
+end
+
+(* TODO: Type annotations *)
+locale variable_substitution_lifting = base: variable_substitution + 
+  variable_substitution where
+     subst = lifted_subst and 
+     id_subst = id_subst and 
+     comp_subst = comp_subst and 
+     vars = lifted_vars 
+  for lifted_subst lifted_vars  +
+  assumes lifted_vars_vars:  "(\<forall>x. lifted_vars (lifted_subst x \<gamma>) = {}) \<longleftrightarrow> (\<forall>x. vars (x \<cdot> \<gamma>) = {})"
+begin
+
+lemma is_ground_subst_iff [simp]: "is_ground_subst \<gamma> \<longleftrightarrow> base.is_ground_subst \<gamma>"
+  unfolding is_ground_subst_def  base.is_ground_subst_def
+  using lifted_vars_vars
+  by presburger
+
+end
+
+end
